% NOTE: Check proof

% foreword
For a topological space $X$, we define the \defterm{cone} of $X$ to be 
\[ CX := X \times [0, 1] / X \times \{1\} \]
and for a map $f: A \to B$ the \defterm{mapping cone} of $f$ to be
\[ B \sqcup_f CA := B \sqcup CA / \sim \]
where $(a, 0) \sim b :\iff f(a) = b$.

Similarly, we define the \defterm{cylinder} of $X$ to be
\[ MX := X \times [0, 1] \]
and for a map $f: A \to B$ the \defterm{mapping cylinder} of $f$ to be
\[ B \sqcup_f MA := B \sqcup CA / \sim \]
where $(a, 0) \sim b :\iff f(a) = b$.

% lemma: extending over a mapping cone
\begin{mylemma}
A microbundle $\bb$ over $B$ can be extended to a microbundle over the mapping cone $B \sqcup_f CA$ if and only if $f^*\bb$ is trivial.
\end{mylemma}
% proof
\begin{myproof}
We show both implications.

% =>
``$\implies$''

Let $\bb'$ be an extension of $\bb$ over $B \sqcup_f CA$.
Considering $A \xto{f} B \incl B \sqcup_f CA$, the composition $\iota \circ f$ is null-homotopic with homotopy
\[ H_t(a) := [(a, t)] \]
Note that $H_0(a) = [(a, 0)] = [f(a)] = (\iota \circ f)(a)$ and $H_1(a) = [(a, 1)] = [(\tilde{a}, 1)] = H_1(\tilde{a})$.
From the Homotopy Theorem~\ref{homotopy::theorem} follows that $(\iota \circ f)^*\bb'$ is trivial. 

Since $(\iota \circ f)^*\bb' = f^*(\iota^*\bb') = f^*\bb$, it follows that $f^*\bb$ is trivial.

% <=
``$\impliedby$''

Let $f^*\bb$ be trivial.

In contrast to the mapping cone, there exists a natural retraction from the mapping cylinder to the attached space
\[ \pi: B \sqcup_f MA \to B, \pi([(a, t)]) := f(a) \]
The diagram
\[ A \times \{1\} \incl B \sqcup_f MA \xto{\pi} B \]
equals $f$ if we consider $A = A \times \{1\}$.
It follows that
\[ \pi^*\bb\restr{A \times \{1\}} = (\pi \circ \iota)^*\bb \cong f^*\bb = \mathfrak{e}^n_A\]
is trivial.
From \cref{induced::trivial} and $(a, t) \mapsto (a, 1)$ it follows that $\pi^*\bb\restr{A \times [\frac{1}{2}, 1]}$ is trivial, so
\[ \exists \phi: E(\bb\restr{A \times [\frac{1}{2}, 1]}) \isomto A \times [\frac{1}{2}, 1] \times \R^n \]
Now we explicitly construct our desired extended microbundle $\bundledef{\bb'}{B \sqcup_f CA}{E'}{i'}{j'}$
\begin{itemize}
    \item $E' := E(\bb\restr{A \times [\frac{1}{2}, 1]}) / \phi^{-1}(A \times [\frac{1}{2}, 1] \times \{x\})$ (for every $x \in \R^n$)
    \item $i' := \pi \circ i$ the projection map.
    \item $j'([e]) := [j(e)]$ is well-defined since $[e] = [\tilde{e}] \implies [j(e)] = [j(e')]$
\end{itemize}
We derive the microbundle conditions from 
Now that we have constructed $\bb'$, the prove is complete.
\end{myproof}