% definition
\begin{mystatement}{definition}[induced microbundle]{induced::definition}[58]
    Let $\bb$ be a microbundle over $B$ and let $f: A \to B$ be a map.
    The \defterm{induced microbundle} $\ind{f}\bb$ is a microbundle $\bundle{A}{E_f}{i_f}{j_f}$
    defined as follows:
    \begin{itemize}
        \item $E_f = \{ (a, e) \in A \cross E(\bb) \mid f(a) = j(e) \}$
        \item $i_f(a) = (a, (i \circ f)(a))$
        \item $j_f(a, e) = a$
    \end{itemize}
\end{mystatement}

% fiber bundle
\begin{myparagraph}
    The construction is identical to the one over vector bundles,
    more precisely over fiber bundles (compare to \cite[ch.2,sec.14]{brendon}).
\end{myparagraph}

% proof
\begin{myproof}[that $\ind{f}\bb$ is a microbundle]
    % continuity and compatibility
    Both $i_f$ and $j_f$ are continuous
    since they are composed by continuous functions.
    Additionally, $j_f(i_f(a)) = j_f(a, i(f(a))) = a$ and hence $j_f \circ i_f = id_A$.

    % local triviality
    It remains to be shown that $\ind{f}\bb$ is locally trivial.

    % local triviality :: homeomorphism
    For an arbitrary $a \in A$,
    choose a local trivialization $(U, V, \phi)$ of $i(a)$ in $\bb$.
    We construct a local trivialization of $a$ in $\ind{f}\bb$ as follows:
    \begin{itemize}
        \item $U_f = \inv{f}(U) \sub A$,
        which is an open neighborhood of $a$ since $f$ is continuous
        and $U$ is an open neighborhood of $i(a)$.
        \item $V_f = (U_f \cross V) \cap E_f \sub E_f$,
        which is an open neighborhood of $i_f(a)$
        since both $U' \cross V$ and $E_f$ are open neighborhoods of $i_f(a)$.
        \item $\phi_f: V_f \isomto U_f \cross \R^n$ with $\phi_f(a', e) = (a', \snd{\phi}(e))$
    \end{itemize}
    The existence of an inverse $\inv{\phi_f}(a', v) = (a', \inv{\phi}(f(a'), v))$
    and component-wise continuity for both $\phi_f$ and $\inv{\phi_f}$ show that $\phi_f$ is a homeomorphism.
    
    % local triviality :: commutativity
    Commutativity with $i_f$ and $id \times 0$ is given by
    \[ \phi_f(i_f(a')) = \phi(a', i(f(a'))) = (a', \snd{\phi}(i(f(a')))) = (a', 0) = (id \cross 0)(a') \]
    and with $j_f$ and $\pi_1$ by
    \[ j_f(a', e) = a'  = \pi_1(a', \phi(e)) = \pi_1(\phi_f(a', e)), \]
    which completes the proof.
\end{myproof}