
\begin{mystatement}{definition}[composition microbundle]{normal::composition}[63] Let $\ba$ be a $n$-dimensional microbundle \[ \bundledef{\ba}{A}{E(\ba)}{i_a}{j_a} \] and let $\bb$ be a $n'$-dimensional microbundle \[ \bundledef{\bb}{E(\ba)}{E(\bb)}{i_b}{j_b}. \] The \defterm{composition microbundle} $\ba \circ \bb$ is a $(n + n')$-dimensional microbundle \[ \bundle{A}{E(\bb)}{i}{j} \] where $i = i_b \circ i_a$ and $j = j_a \circ j_b$. \end{mystatement}

\begin{myproof}[that $\ba \circ \bb$ is a microbundle] Both injection and projection maps are continuous as being composed by continuous maps. Additionally, $j \circ i = j_a \circ (j_b \circ i_b) \circ i_a = j_a \circ i_a = id_A$.

It remains to be shown that $\ba \circ \bb$ is locally trivial.

For an arbitrary $a \in A$, choose local trivializations $(U_a, V_a, \phi_a)$ of $a$ in $\ba$ and $(U_b, V_b, \phi_b)$ of $i_a(a)$ in $\bb$. Note that both $U_b$ and $V_a$ are open neighborhoods of $i_a(a)$.

Without loss of generality, we may assume that $V_a = U_b$:

`$\sub$': Modify $U_a$ such that \[ U_a \cross \ball[\eps] \sub \phi_a(V_a \cap U_b) \] for a sufficiently small $\eps > 0$ and let \[ V_a = \inv{\phi_a}(U_a \cross \ball[\eps]) \sub V_a \cap U_b. \] Composing $\phi_a$ with $\mu_\eps: \ball[\eps] \isomto \R^n$ yields a local trivialization of $a$ in $\ba$ such that $V_a \sub U_a$.

`$\bus$': Restrict $U_b$ to $V_a \cap U_b$ and $V_b$ to $\inv{\phi_b}((V_a \cap U_b) \cross \R^{n'})$.

We have local-trivialization $(U_a, V_b, \phi)$ of $a$ in $\ba \circ \bb$ given by \[ \phi: V_b \xto{\phi_b} U_b \cross \R^{n'} = V_a \cross \R^{n'} \xto{\phi_a \cross id} (U_a \cross \R^{n}) \cross \R^{n'} = U_a \cross \R^{n + n'}, \] which is a homeomorphism since it's composed by homeomorphisms.

Furthermore, $\phi$ commutes with the injection and projection maps, as the following equations show: \begin{gather} \begin{split} \phi(i(a)) = \phi(i_b(i_a(a))) = (\phi_a(i_a(a)), \snd{\phi_b}(i_b(i_a(a)))) \\ = (\snd{\phi_a}(i_a(a)), 0) = (a, (0, 0)) = (id_{U_a} \cross 0)(a)  \end{split} \\ j(e) = j_a(j_b(e)) = \pi_1(j_a(j_b(e)), \snd{\phi}(e)) = \pi_1(\phi(e)) \end{gather} This completes the proof. \end{myproof}