% definition
\begin{mydefinition}{suspension::whitney}{}
    The \defterm{whitney sum} of two rooted microbundles $\bb$ and $\bb'$ over $B$
    is the initial whitney sum $\whitney{\bb}{\bb'}$ together with the rooting
    \[ \germdef{\whitney{R}{R'}}{(\whitney{\bb}{\bb'})\restr{b_0}}{\whitney{\be[n_1]{b_0}}{\be[n_2]{b_0}} = \be[n_1 + n_1]{b_0}}. \]
\end{mydefinition}

% lemma
\begin{mylemma}{suspension::compatability}{}   
    The following non-rooted isomorphy holds
    for rooted microbundles $\ba$ and $\ba'$ over $A$
    and $\bb$ and $\bb'$ over $B$: 
    \[
        \whitney{(\ba \vee \bb)}{(\ba' \vee \bb')}
        \cong (\whitney{\ba}{\ba'}) \vee (\whitney{\bb}{\bb'})
    \]
\end{mylemma}
\begin{myproof}
    Consider the equation
    \[ E(\whitney{(\ba \vee \bb)}{(\ba' \vee \bb')}) \]
    \[ = \set{(e, e') \in E(\ba \vee \bb) \times E(\ba' \vee \bb')}{j(e) = j'(e')} \]
    \[ = \set{(e, e') \in ((E(\ba) \sqcup E(\bb)) / \sim) \times ((E(\ba') \sqcup E(\bb')) / \sim')}{j(e) = j'(e')} \]
    \[ = (\set{(e, e') \in E(\ba) \times E(\ba')}{j_a(e) = j_{a'}(e')} \sqcup \]
    \[ \set{(e, e') \in E(\bb) \times E(\bb')}{j_b(e) = j_{b'}(e')}) / \backsim \]
    \[ = (E(\whitney{\ba}{\ba'}) \sqcup E(\whitney{\bb}{\bb'})) / \backsim \]
    \[ = E((\whitney{\ba}{\ba'}) \vee (\whitney{\bb}{\bb'})) \]
    where $(e_a, e_a') \backsim (e_b, e_b') \iff e_a \sim e_b \land e_a' \sim' e_b'$.
    Here, the equivalence relations $\sim$ and $\sim'$ denote the ones
    used in the construction of the corresponding wedge sums.

    Additionally, the injection
    \[ i_\oplus(a) = (i_a(a), i_a'(a)) = i_\vee(a) \text{ (symmetrical for $b$)}\]
    and projection maps
    \[ j_\oplus(e, e') = j(e) =  j_\vee(e) \]
    are equal.
    Here, $i_\oplus$ and $j_\oplus$ denote the injection and projection maps for
    \[ \whitney{(\ba \vee \bb)}{(\ba' \vee \bb')} \]
    and $i_\vee$ and $j_\vee$ denote the injection and projection maps for
    \[ (\whitney{\ba}{\ba'}) \vee (\whitney{\bb}{\bb'}). \]
    It follows that the two microbundles are isomorphic.
\end{myproof}