\begin{myparagraph} Let $r: B \isomto B$ denote the `reflection' given by \[ r([x, t]) = [x, 1 - t] \] and let $c: B \vee B \to B$ denote the identity on the first summand and $r$ on the second summand, i.e, \[ c(b, i) = \case{b}{r(b)}{i = 1}. \] \end{myparagraph}

\begin{mystatement}{lemma}{suspension::reflection}[70] The induced microbundle $\ind{\phi}(\bb \vee \ind{r}\bb)$ is trivial. \end{mystatement}

\begin{myproof} The composition $c \circ \phi$ is null-homotopic via the homotopy $H: B \cross \I \to B$ given by \[ H([x, t], s) = f(\phi(x, t \cdot s)). \] Applying \myintref{homotopy::theorem} yields $\ind{\phi}(\ind{c}\bb) \cong \ind{(c \circ \phi)}\bb \cong \ind{c_{B, b_0}}\bb \cong \be{B}$ as rooted-isomorphy. Note that the induced microbundle preserves rootings (see \myintref{suspension::induced}). By applying the previous lemma, it follows that \[ \ind{\phi}(\bb \vee \ind{r}\bb) = \ind{\phi}(\ind{(id \cup r)}(\bb \vee \bb)) = \ind{\phi}(\ind{c}\bb) \] and hence $\ind{\phi}(\bb \vee \ind{r}\bb) \cong \be{B}$. \end{myproof}