% lemma
\begin{mystatement}{lemma}{suspension::triviality}
    The following (non-rooted) isomorphy holds:
    \[ \ind{\phi}(\bb \vee \be{B}) \cong \bb \cong \ind{\phi}(\be{B} \vee \bb) \]
\end{mystatement}

% proof
\begin{myproof}
    We prove the lemma in two steps.
    \begin{steps}
        % step 1
        \step{$\ind{c_1}\bb \cong \bb \vee \be{B}$}
        
        % representative
        Let $E(\bb \vee \be{B})$ be constructed via 
        the representative $f: V \to b_0 \cross \R^n$ for $R$.

        Without loss of generality, we may assume that
        $V = E(\bbb)$ by removing the closed set $E(\bbb) - V$ from $E(\bb)$ if necessary.

        % homeomorphy
        Consider $\psi: E(\ind{c_1}\bb) \isomto E(\bb \vee \be{B})$ given by
        \[ \psi((b, i), e) = \case{e}{(b, \snd{f}(e))}{i = 1} \]
        Note that $\psi$ is well-defined, because
        \[ \psi((b_0, 1), e) = e = f(e) = (b_0, \snd{f}(e)) = \psi((b_0, 2), e). \]
        and that $\psi$ is well-defined, because

        Additionally, $\psi$ is a homeomorphism as both of its summands are homeomorphisms.

        % commutativity
        Finally, it remains to be shown that $\psi$
        commutes with the injection and projection maps from $\ind{c_1}\bb$ and $\bb \vee \be{B}$.
        To check this, consider the following equations:
        \begin{align}
            &\psi(i_{c_1}(b, i)) = \casenif{\psi((b, 1), i(b)) = i(b) = i_\vee(b, 1)}{\psi((b, 2), i(b_0)) = f(i(b)) = (b, 0) = (id \cross 0)(b) = i_\vee(b, 2)} \\
            &j_{c_1}((b, i), e) = \casenif{j(e) = j_\vee(e) = j_\vee(\psi((b, 1), e))}{(b, 2) = \pi_1(\psi((b, 2), e)) = j_\vee(\psi((b, 2), e))}
        \end{align}
        
        % step 2
        \step{$\ind{\phi}(\bb \vee \be{B}) \cong \bb$}

        Using the fact that $c_1 \circ \phi = id_{B \vee B}$, we conclude that
        \[ \ind{\phi}(\bb \vee \be{B}) \cong \ind{\phi}(\ind{c_1}\bb) \cong \ind{(c_1 \circ \phi)}\bb \cong \bb. \]
        For reasons of symmetry, it follows that $\bb \cong \ind{\phi}(\be{B} \vee \bb)$.
        This completes the proof.
    \end{steps}
\end{myproof}